logic.lean
@@ -1,30 +1,74 @@
-import .syntax .etc .props
+import .syntax .etc .props .evaluation
 
 -- instantiation
 
-constant prop.instantiated_p: prop → qfprop
+constant prop.instantiated: prop → vc
 
-constant prop.instantiated_n: prop → qfprop
+constant prop.instantiated_n: prop → vc
 
-axiom instantiated.not {P: prop}: P.not.instantiated_p = P.instantiated_n.not
+mutual def prop.erased, prop.erased_n
 
-def prop.erased_p: prop → qfprop
-| (prop.term t)        := qfprop.term t
-| (prop.not P)         := qfprop.not P.erased_n
-| (prop.and P₁ P₂)     := P₁.erased_p && P₂.erased_p
-| (prop.or P₁ P₂)      := P₁.erased_p || P₂.erased_p
-| (prop.pre t₁ t₂)     := qfprop.pre t₁ t₂
-| (prop.pre₁ op t)     := qfprop.pre₁ op t
-| (prop.pre₂ op t₁ t₂) := qfprop.pre₂ op t₁ t₂
-| (prop.post t₁ t₂)    := qfprop.post t₁ t₂
-| (prop.call t₁ t₂)    := qfprop.call t₁ t₂
-| (prop.forallc x t P) := qfprop.forallc x t p.to_propctx
-| (prop.exist x P)     := qfprop.exist x p.to_propctx
+with prop.erased: prop → vc
+| (prop.term t)        := vc.term t
+| (prop.not P)         := have h: P.size + 1 < P.size + 2, from lt_of_add_one,
+                          have P.size + 2 = 2 + P.size, from add_comm P.size 2,
+                          have P.size + 1 < 2 + P.size, from this ▸ h,
+                          vc.not P.erased_n
+| (prop.and P₁ P₂)     := have P₁.size < (P₁ && P₂).size, from lt_of_add.left,
+                          have P₂.size < (P₁ && P₂).size, from lt_of_add.right,
+                          P₁.erased && P₂.erased
+| (prop.or P₁ P₂)      := have P₁.size < (P₁ || P₂).size, from lt_of_add.left,
+                          have P₂.size < (P₁ || P₂).size, from lt_of_add.right,
+                          P₁.erased || P₂.erased
+| (prop.pre t₁ t₂)     := vc.pre t₁ t₂
+| (prop.pre₁ op t)     := vc.pre₁ op t
+| (prop.pre₂ op t₁ t₂) := vc.pre₂ op t₁ t₂
+| (prop.post t₁ t₂)    := vc.post t₁ t₂
+| (prop.call _ _)      := vc.term value.true
+| (prop.forallc x t P) := have P.size < (prop.forallc x t P).size, from lt_of_add_one,
+                          vc.univ x P.erased
+| (prop.exis x P)      := vc.term value.false -- TODO: look into this
+
+with prop.erased_n: prop → vc
+| (prop.term t)        := vc.term t
+| (prop.not P)         := have h: P.size + 1 < P.size + 2, from lt_of_add_one,
+                          have P.size + 2 = 2 + P.size, from add_comm P.size 2,
+                          have P.size + 1 < 2 + P.size, from this ▸ h,
+                          vc.not P.erased
+| (prop.and P₁ P₂)     := have P₁.size < (P₁ && P₂).size, from lt_of_add.left,
+                          have P₂.size < (P₁ && P₂).size, from lt_of_add.right,
+                          P₁.erased_n && P₂.erased_n
+| (prop.or P₁ P₂)      := have P₁.size < (P₁ || P₂).size, from lt_of_add.left,
+                          have P₂.size < (P₁ || P₂ ).size, from lt_of_add.right,
+                          P₁.erased_n || P₂.erased_n
+| (prop.pre t₁ t₂)     := vc.pre t₁ t₂
+| (prop.pre₁ op t)     := vc.pre₁ op t
+| (prop.pre₂ op t₁ t₂) := vc.pre₂ op t₁ t₂
+| (prop.post t₁ t₂)    := vc.post t₁ t₂
+| (prop.call _ _)      := vc.term value.true
+| (prop.forallc x t P) := vc.term value.true
+| (prop.exis x P)      := have P.size < P.size + 1, from lt_of_add_one,
+                          vc.not (vc.univ x (vc.not P.erased_n))
+
+inductive no_instantiations: prop -> Prop
+| term {t: term}                 : no_instantiations t
+| not {P: prop}                  : no_instantiations P → no_instantiations (prop.not P)
+| and {P₁ P₂: prop}              : no_instantiations P₁ → no_instantiations (prop.and P₁ P₂)
+| or {P₁ P₂: prop}               : no_instantiations P₂ → no_instantiations (prop.or P₁ P₂)
+| pre {t₁ t₂: term}              : no_instantiations (prop.pre t₁ t₂)
+| pre₁ {t: term} {op: unop}      : no_instantiations (prop.pre₁ op t)
+| pre₂ {t₁ t₂: term} {op: binop} : no_instantiations (prop.pre₂ op t₁ t₂)
+| post {t₁ t₂: term}             : no_instantiations (prop.post t₁ t₂)
+
+axiom not_dist_instantiated {P: prop}:
+  P.not.instantiated = P.instantiated_n.not
 
  -- propositions without quantifiers or call triggers do not participate in instantiations
-axiom and_dist_of_no_instantiations {P: prop} {Q: qfprop}: (P && Q).instantiated_p = P.instantiated_p && Q
+axiom and_dist_of_no_instantiations {P Q: prop}:
+  no_instantiations Q → ((P && Q).instantiated = P.instantiated && Q.erased)
 
-axiom or_dist_of_no_instantiations {P: prop} {Q: qfprop}: (P || Q).instantiated_p = P.instantiated_p || Q
+axiom or_dist_of_no_instantiations {P Q: prop}:
+  no_instantiations Q → ((P || Q).instantiated = P.instantiated || Q.erased)
 
 -- substitution
 
@@ -34,6 +78,12 @@ def term.subst (x: var) (v: value): term → term
 | (term.unop op t)      := term.unop op t.subst
 | (term.binop op t₁ t₂) := term.binop op t₁.subst t₂.subst
 | (term.app t₁ t₂)      := term.app t₁.subst t₂.subst
+
+def term.subst_env: env → term → term
+| env.empty t := t
+| (σ[x↦v]) t :=
+    have σ.size < (σ[x ↦ v].size), from lt_of_add_one,
+    term.subst_env σ (term.subst x v t)
 
 def spec.subst (x: var) (v: value): spec → spec
 | (spec.term t) :=
@@ -60,54 +110,95 @@ def spec.subst_env: env → spec → spec
 | env.empty R := R
 | (σ[x↦v]) R :=
     have σ.size < (σ[x ↦ v].size), from lt_of_add_one,
-    spec.subst x v (spec.subst_env σ R)
+    spec.subst_env σ (spec.subst x v R)
 
-def qfprop.subst (x: var) (v: value): qfprop → qfprop
-| (qfprop.term t)        := term.subst x v t
-| (qfprop.not P)         := qfprop.not P.subst
-| (qfprop.and P Q)       := P.subst && Q.subst
-| (qfprop.or P Q)        := P.subst || Q.subst
-| (qfprop.pre t₁ t₂)     := qfprop.pre (term.subst x v t₁) (term.subst x v t₂)
-| (qfprop.pre₁ op t)     := qfprop.pre₁ op (term.subst x v t)
-| (qfprop.pre₂ op t₁ t₂) := qfprop.pre₂ op (term.subst x v t₁) (term.subst x v t₂)
-| (qfprop.post t₁ t₂)    := qfprop.post (term.subst x v t₁) (term.subst x v t₂)
+def vc.subst (x: var) (v: value): vc → vc
+| (vc.term t)        := term.subst x v t
+| (vc.not P)         := vc.not P.subst
+| (vc.and P Q)       := P.subst && Q.subst
+| (vc.or P Q)        := P.subst || Q.subst
+| (vc.pre t₁ t₂)     := vc.pre (term.subst x v t₁) (term.subst x v t₂)
+| (vc.pre₁ op t)     := vc.pre₁ op (term.subst x v t)
+| (vc.pre₂ op t₁ t₂) := vc.pre₂ op (term.subst x v t₁) (term.subst x v t₂)
+| (vc.post t₁ t₂)    := vc.post (term.subst x v t₁) (term.subst x v t₂)
+| (vc.univ y P)      := vc.univ y (if x = y then P else P.subst)
 
-def qfprop.subst_env: env → qfprop → qfprop
+def vc.subst_env: env → vc → vc
 | env.empty P := P
 | (σ[x↦v]) P :=
     have σ.size < (σ[x ↦ v].size), from lt_of_add_one,
-    qfprop.subst x v (qfprop.subst_env σ P)
+    vc.subst_env σ (vc.subst x v P)
 
 -- validity
 
-inductive valid : qfprop → Prop
+inductive valid : vc → Prop
 notation `⊨` p: 100 := valid p
 
-| tru: ⊨ value.true
+| tru:
+  ⊨ value.true
 
-| eq {t: term}: ⊨ term.binop binop.eq t t
+| unop {op: unop} {vₓ v: value}:
+  op vₓ = some v →
+  ⊨ term.binop binop.eq (term.unop op vₓ) v
 
-| and {Q P: qfprop}: ⊨ P → ⊨ Q → ⊨ (P && Q)
+| binop {op: binop} {v₁ v₂ v: value}:
+  op v₁ v₂ = some v →
+  ⊨ term.binop binop.eq (term.binop op v₁ v₂) v
 
-| orl {Q P: qfprop}: ⊨ P → ⊨ (P || Q)
+| app {vₓ v: value} {σ σ': env} {f x y: var} {R S: spec} {e: exp}:
+  (σ[x↦vₓ], e) ⟶* (σ', exp.return y) →
+  (σ' y = some v) →
+  ⊨ term.binop binop.eq (term.app (value.func f x R S e σ) vₓ) v
 
-| orr {Q P: qfprop}: ⊨ Q → ⊨ (P || Q)
+| and {P Q: vc}:
+  ⊨ P →
+  ⊨ Q →
+  ⊨ (P && Q)
 
-| mp {Q P: qfprop}: ⊨ qfprop.implies P Q → ⊨ P → ⊨ Q
+| orl {P Q: vc}:
+  ⊨ P →
+  ⊨ (P || Q)
+
+| orr {P Q: vc}:
+  ⊨ Q →
+  ⊨ (P || Q)
+
+| pre {vₓ: value} {σ: env} {f x y: var} {R S: spec} {e: exp}:
+  ⊨ vc.subst_env (σ[x↦vₓ][f↦value.func f x R S e σ]) R.to_prop.instantiated →
+  ⊨ vc.pre (value.func f x R S e σ) vₓ
+
+| pre₁ {vₓ v: value} {op: unop}:
+  (∃v, op vₓ = some v) →
+  ⊨ vc.pre₁ op vₓ
+
+| pre₂ {v₁ v₂ v: value} {op: binop}:
+  (∃v, op v₁ v₂ = v) →
+  ⊨ vc.pre₂ op v₁ v₂
+
+| post {vₓ: value} {σ σ': env} {f x y: var} {R S: spec} {e: exp}:
+  (σ[x↦vₓ], e) ⟶* (σ', exp.return y) →
+  ⊨ vc.subst_env (σ[x↦vₓ][f↦value.func f x R S e σ]) (spec.implies R S).to_prop.instantiated →
+  ⊨ vc.post (value.func f x R S e σ) vₓ
+
+| univ {x: var} {P: vc}:
+  (∀v, ⊨ vc.subst x v P) →
+  ⊨ vc.univ x P
 
 notation `⊨` p: 100 := valid p
-notation σ `⊨` p: 100 := valid (qfprop.subst_env σ p)
+notation σ `⊨` p: 100 := valid (vc.subst_env σ p)
+
+axiom valid.mp  {P Q: vc}: ⊨ vc.implies P Q → ⊨ P → ⊨ Q
 
 -- axioms about instantiation
 
-axiom instantiated_p_of_erased_p {σ: env} {P: prop} : σ ⊨ P.erased_p → σ ⊨ P.instantiated_p
-axiom instantiated_n_of_instantiated_p {σ: env} {P: prop} : σ ⊨ P.instantiated_p → σ ⊨ P.instantiated_n
+axiom instantiated_p_of_erased_p {σ: env} {P: prop} : σ ⊨ P.erased → σ ⊨ P.instantiated
+axiom instantiated_n_of_instantiated_p {σ: env} {P: prop} : σ ⊨ P.instantiated → σ ⊨ P.instantiated_n
 axiom erased_n_of_instantiated_n {σ: env} {P: prop} : σ ⊨ P.instantiated_n → σ ⊨ P.erased_n
 
 -- notation ⟪ P ⟫
 
 @[reducible]
-def VC(P: prop) := ∀ (σ: env), σ ⊨ P.instantiated_p
+def VC(P: prop) := ∀ (σ: env), σ ⊨ P.instantiated
 
 notation `⟪` P `⟫`: 100 := VC P
 
@@ -200,31 +291,31 @@ lemma free_of_subst_spec {R: spec} {x y: var} {v: value}:
   --     have x ≠ y ∧ free_in_prop x S₁.to_prop, from S₁_ih this,
   --     show x ≠ y ∧ free_in_prop x S₁.not.to_prop, from ⟨this.left, free_in_prop.not this.right⟩
   --   ),
-  --   show x ≠ y ∧ free_in_prop x (S₂ & S₃).to_prop, from (
-  --     have spec.subst y v (spec.and S₂ S₃) = (spec.subst y v S₂ & spec.subst y v S₃), by unfold spec.subst,
-  --     have x_free_in_and': free_in_prop x (spec.subst y v S₂ & spec.subst y v S₃).to_prop, from this ▸ x_free_in_subst,
+  --   show x ≠ y ∧ free_in_prop x (S₂ && S₃).to_prop, from (
+  --     have spec.subst y v (spec.and S₂ S₃) = (spec.subst y v S₂ && spec.subst y v S₃), by unfold spec.subst,
+  --     have x_free_in_and': free_in_prop x (spec.subst y v S₂ && spec.subst y v S₃).to_prop, from this ▸ x_free_in_subst,
   --     have (spec.and (spec.subst y v S₂) (spec.subst y v S₃)).to_prop
-  --        = ((spec.subst y v S₂).to_prop & (spec.subst y v S₃).to_prop),
+  --        = ((spec.subst y v S₂).to_prop && (spec.subst y v S₃).to_prop),
   --     by unfold spec.to_prop,
-  --     have free_in_prop x ((spec.subst y v S₂).to_prop & (spec.subst y v S₃).to_prop), from this ▸ x_free_in_and',
+  --     have free_in_prop x ((spec.subst y v S₂).to_prop && (spec.subst y v S₃).to_prop), from this ▸ x_free_in_and',
   --     have free_in_prop x (spec.subst y v S₂).to_prop ∨ free_in_prop x (spec.subst y v S₃).to_prop,
   --     from free_in_prop.and.inv this,
   --     or.elim this (
   --       assume : free_in_prop x (spec.subst y v S₂).to_prop,
   --       have x ≠ y ∧ free_in_prop x S₂.to_prop, from S₂_ih this,
-  --       show x ≠ y ∧ free_in_prop x (S₂ & S₃).to_prop, from ⟨this.left, free_in_prop.and₁ this.right⟩
+  --       show x ≠ y ∧ free_in_prop x (S₂ && S₃).to_prop, from ⟨this.left, free_in_prop.and₁ this.right⟩
   --     ) (
   --       assume : free_in_prop x (spec.subst y v S₃).to_prop,
   --       have x ≠ y ∧ free_in_prop x S₃.to_prop, from S₃_ih this,
-  --       show x ≠ y ∧ free_in_prop x (S₂ & S₃).to_prop, from ⟨this.left, free_in_prop.and₂ this.right⟩
+  --       show x ≠ y ∧ free_in_prop x (S₂ && S₃).to_prop, from ⟨this.left, free_in_prop.and₂ this.right⟩
   --     )
   --   ),
   --   show x ≠ y ∧ free_in_prop x (spec.or S₄ S₅).to_prop, from (
-  --     have spec.subst y v (spec.or S₄ S₅) = spec.or (spec.subst y v S₄) (spec.subst y v S₅), by unfold spec.subst,
+  --     have spec.subst y v (spec.or S₄ S₅) = (spec.subst y v S₄) || (spec.subst y v S₅), by unfold spec.subst,
   --     have x_free_in_or': free_in_prop x (spec.or (spec.subst y v S₄) (spec.subst y v S₅)).to_prop,
   --     from this ▸ x_free_in_subst,
   --     have (spec.or (spec.subst y v S₄) (spec.subst y v S₅)).to_prop
-  --        = (prop.or (spec.subst y v S₄).to_prop (spec.subst y v S₅).to_prop),
+  --        = ((spec.subst y v S₄).to_prop || (spec.subst y v S₅).to_prop),
   --     by unfold spec.to_prop,
   --     have free_in_prop x (prop.or (spec.subst y v S₄).to_prop (spec.subst y v S₅).to_prop),
   --     from this ▸ x_free_in_or',
@@ -245,15 +336,15 @@ lemma free_of_subst_spec {R: spec} {x y: var} {v: value}:
   --       have h₁: spec.subst y v (spec.func f fx S₆ S₇) = spec.func (term.subst y v f) fx S₆ S₇,
   --       by { unfold spec.subst, simp * },
   --       let forallp := (prop.implies S₆.to_prop (prop.pre (term.subst y v f) fx)
-  --                     & prop.implies (S₆.to_prop & prop.post (term.subst y v f) fx) S₇.to_prop) in
+  --                     && prop.implies (S₆.to_prop && prop.post (term.subst y v f) fx) S₇.to_prop) in
   --       have h₂: (spec.func (term.subst y v f) fx S₆ S₇).to_prop =
-  --                (term.unop unop.isFunc (term.subst y v f) & prop.forallc fx (term.subst y v f) forallp),
+  --                (term.unop unop.isFunc (term.subst y v f) && prop.forallc fx (term.subst y v f) forallp),
   --       by unfold spec.to_prop,
   --       let forallp' := (prop.implies S₆.to_prop (prop.pre f fx)
-  --                       & prop.implies (S₆.to_prop & prop.post f fx) S₇.to_prop) in
-  --       have h₃: (spec.func f fx S₆ S₇).to_prop = (term.unop unop.isFunc f & prop.forallc fx f forallp'),
+  --                       && prop.implies (S₆.to_prop && prop.post f fx) S₇.to_prop) in
+  --       have h₃: (spec.func f fx S₆ S₇).to_prop = (term.unop unop.isFunc f && prop.forallc fx f forallp'),
   --       by unfold spec.to_prop,
-  --       have free_in_prop x (term.unop unop.isFunc (term.subst y v f) & prop.forallc fx (term.subst y v f) forallp),
+  --       have free_in_prop x (term.unop unop.isFunc (term.subst y v f) && prop.forallc fx (term.subst y v f) forallp),
   --       from h₂ ▸ h₁ ▸ x_free_in_subst,
   --       have free_in_prop x (term.unop unop.isFunc (term.subst y v f))
   --          ∨ free_in_prop x (prop.forallc fx (term.subst y v f) forallp),
@@ -266,7 +357,7 @@ lemma free_of_subst_spec {R: spec} {x y: var} {v: value}:
   --         have free_in_term x f, from (free_of_subst_term this).right,
   --         have free_in_term x (term.unop unop.isFunc f), from free_in_term.unop this,
   --         have free_in_prop x (term.unop unop.isFunc f), from free_in_prop.term this,
-  --         have free_in_prop x (term.unop unop.isFunc f & prop.forallc fx f forallp'), from free_in_prop.and₁ this,
+  --         have free_in_prop x (term.unop unop.isFunc f && prop.forallc fx f forallp'), from free_in_prop.and₁ this,
   --         -- have free_in_prop x (spec.func f fx S₆ S₇).to_prop, from h₃ ▸ this,
   --         show x ≠ y ∧ free_in_prop x (spec.func f fx S₆ S₇).to_prop, from ⟨x_neq_y, this⟩
   --       ) (
@@ -279,7 +370,7 @@ lemma free_of_subst_spec {R: spec} {x y: var} {v: value}:
   --           have free_in_term x f, from (free_of_subst_term this).right,
   --           have free_in_term x (term.unop unop.isFunc f), from free_in_term.unop this,
   --           have free_in_prop x (term.unop unop.isFunc f), from free_in_prop.term this,
-  --           have free_in_prop x (term.unop unop.isFunc f & prop.forallc fx f forallp'), from free_in_prop.and₁ this,
+  --           have free_in_prop x (term.unop unop.isFunc f && prop.forallc fx f forallp'), from free_in_prop.and₁ this,
   --           have free_in_prop x (spec.func f fx S₆ S₇).to_prop, from h₃ ▸ this,
   --           show x ≠ y ∧ free_in_prop x (spec.func f fx S₆ S₇).to_prop, from ⟨x_neq_y, this⟩
   --         ) (
@@ -292,7 +383,7 @@ lemma free_of_subst_spec {R: spec} {x y: var} {v: value}:
   --               have free_in_prop x (prop.implies S₆.to_prop (prop.pre f fx)), from free_in_prop.or₁ this,
   --               have free_in_prop x forallp', from free_in_prop.and₁ this,
   --               have free_in_prop x (prop.forallc fx f forallp'), from free_in_prop.forallc₂ x_neq_fx this,
-  --               have free_in_prop x (term.unop unop.isFunc f & prop.forallc fx f forallp'), from free_in_prop.and₂ this,
+  --               have free_in_prop x (term.unop unop.isFunc f && prop.forallc fx f forallp'), from free_in_prop.and₂ this,
   --               have free_in_prop x (spec.func f fx S₆ S₇).to_prop, from h₃ ▸ this,
   --               show x ≠ y ∧ free_in_prop x (spec.func f fx S₆ S₇).to_prop, from ⟨x_neq_y, this⟩
   --             ) (
@@ -302,7 +393,7 @@ lemma free_of_subst_spec {R: spec} {x y: var} {v: value}:
   --                 have free_in_term x f, from (free_of_subst_term this).right,
   --                 have free_in_term x (term.unop unop.isFunc f), from free_in_term.unop this,
   --                 have free_in_prop x (term.unop unop.isFunc f), from free_in_prop.term this,
-  --                 have free_in_prop x (term.unop unop.isFunc f & prop.forallc fx f forallp'), from free_in_prop.and₁ this,
+  --                 have free_in_prop x (term.unop unop.isFunc f && prop.forallc fx f forallp'), from free_in_prop.and₁ this,
   --                 have free_in_prop x (spec.func f fx S₆ S₇).to_prop, from h₃ ▸ this,
   --                 show x ≠ y ∧ free_in_prop x (spec.func f fx S₆ S₇).to_prop, from ⟨x_neq_y, this⟩
   --               ) (
@@ -313,17 +404,17 @@ lemma free_of_subst_spec {R: spec} {x y: var} {v: value}:
   --             )
   --           )
   --           (
-  --             assume : free_in_prop x (prop.implies (S₆.to_prop & prop.post (term.subst y v f) fx)
+  --             assume : free_in_prop x (prop.implies (S₆.to_prop && prop.post (term.subst y v f) fx)
   --                                                    S₇.to_prop),
   --             or.elim (free_in_prop.implies.inv this) (
-  --               assume : free_in_prop x (S₆.to_prop & prop.post (term.subst y v f) fx),
+  --               assume : free_in_prop x (S₆.to_prop && prop.post (term.subst y v f) fx),
   --               or.elim (free_in_prop.and.inv this) (
   --                 assume : free_in_prop x S₆.to_prop,
   --                 have free_in_prop x S₆.to_prop.not, from free_in_prop.not this,
   --                 have free_in_prop x (prop.implies S₆.to_prop (prop.pre f fx)), from free_in_prop.or₁ this,
   --                 have free_in_prop x forallp', from free_in_prop.and₁ this,
   --                 have free_in_prop x (prop.forallc fx f forallp'), from free_in_prop.forallc₂ x_neq_fx this,
-  --                 have free_in_prop x (term.unop unop.isFunc f & prop.forallc fx f forallp'), from free_in_prop.and₂ this,
+  --                 have free_in_prop x (term.unop unop.isFunc f && prop.forallc fx f forallp'), from free_in_prop.and₂ this,
   --                 have free_in_prop x (spec.func f fx S₆ S₇).to_prop, from h₃ ▸ this,
   --                 show x ≠ y ∧ free_in_prop x (spec.func f fx S₆ S₇).to_prop, from ⟨x_neq_y, this⟩
   --               ) (
@@ -333,7 +424,7 @@ lemma free_of_subst_spec {R: spec} {x y: var} {v: value}:
   --                   have free_in_term x f, from (free_of_subst_term this).right,
   --                   have free_in_term x (term.unop unop.isFunc f), from free_in_term.unop this,
   --                   have free_in_prop x (term.unop unop.isFunc f), from free_in_prop.term this,
-  --                   have free_in_prop x (term.unop unop.isFunc f & prop.forallc fx f forallp'), from free_in_prop.and₁ this,
+  --                   have free_in_prop x (term.unop unop.isFunc f && prop.forallc fx f forallp'), from free_in_prop.and₁ this,
   --                   have free_in_prop x (spec.func f fx S₆ S₇).to_prop, from h₃ ▸ this,
   --                   show x ≠ y ∧ free_in_prop x (spec.func f fx S₆ S₇).to_prop, from ⟨x_neq_y, this⟩
   --                 ) (
@@ -344,11 +435,11 @@ lemma free_of_subst_spec {R: spec} {x y: var} {v: value}:
   --               )
   --             ) (
   --               assume : free_in_prop x S₇.to_prop,
-  --               have free_in_prop x (prop.implies (S₆.to_prop & prop.post f fx)
+  --               have free_in_prop x (prop.implies (S₆.to_prop && prop.post f fx)
   --                                                  S₇.to_prop), from free_in_prop.or₂ this,
   --               have free_in_prop x forallp', from free_in_prop.and₂ this,
   --               have free_in_prop x (prop.forallc fx f forallp'), from free_in_prop.forallc₂ x_neq_fx this,
-  --               have free_in_prop x (term.unop unop.isFunc f & prop.forallc fx f forallp'), from free_in_prop.and₂ this,
+  --               have free_in_prop x (term.unop unop.isFunc f && prop.forallc fx f forallp'), from free_in_prop.and₂ this,
   --               have free_in_prop x (spec.func f fx S₆ S₇).to_prop, from h₃ ▸ this,
   --               show x ≠ y ∧ free_in_prop x (spec.func f fx S₆ S₇).to_prop, from ⟨x_neq_y, this⟩
   --             )
@@ -360,16 +451,16 @@ lemma free_of_subst_spec {R: spec} {x y: var} {v: value}:
   --          = spec.func (term.subst y v f) fx (spec.subst y v S₆) (spec.subst y v S₇),
   --       by { unfold spec.subst, simp * },
   --       let forallp := (prop.implies (spec.subst y v S₆).to_prop (prop.pre (term.subst y v f) fx)
-  --                     & prop.implies ((spec.subst y v S₆).to_prop & prop.post (term.subst y v f) fx)
+  --                     && prop.implies ((spec.subst y v S₆).to_prop && prop.post (term.subst y v f) fx)
   --                                    (spec.subst y v S₇).to_prop) in
   --       have h₂: (spec.func (term.subst y v f) fx (spec.subst y v S₆) (spec.subst y v S₇)).to_prop =
-  --                (term.unop unop.isFunc (term.subst y v f) & prop.forallc fx (term.subst y v f) forallp),
+  --                (term.unop unop.isFunc (term.subst y v f) && prop.forallc fx (term.subst y v f) forallp),
   --       by unfold spec.to_prop,
   --       let forallp' := (prop.implies S₆.to_prop (prop.pre f fx)
-  --                       & prop.implies (S₆.to_prop & prop.post f fx) S₇.to_prop) in
-  --       have h₃: (spec.func f fx S₆ S₇).to_prop = (term.unop unop.isFunc f & prop.forallc fx f forallp'),
+  --                       && prop.implies (S₆.to_prop && prop.post f fx) S₇.to_prop) in
+  --       have h₃: (spec.func f fx S₆ S₇).to_prop = (term.unop unop.isFunc f && prop.forallc fx f forallp'),
   --       by unfold spec.to_prop,
-  --       have free_in_prop x (term.unop unop.isFunc (term.subst y v f) & prop.forallc fx (term.subst y v f) forallp),
+  --       have free_in_prop x (term.unop unop.isFunc (term.subst y v f) && prop.forallc fx (term.subst y v f) forallp),
   --       from h₂ ▸ h₁ ▸ x_free_in_subst,
   --       have free_in_prop x (term.unop unop.isFunc (term.subst y v f))
   --          ∨ free_in_prop x (prop.forallc fx (term.subst y v f) forallp),
@@ -382,7 +473,7 @@ lemma free_of_subst_spec {R: spec} {x y: var} {v: value}:
   --         have free_in_term x f, from (free_of_subst_term this).right,
   --         have free_in_term x (term.unop unop.isFunc f), from free_in_term.unop this,
   --         have free_in_prop x (term.unop unop.isFunc f), from free_in_prop.term this,
-  --         have free_in_prop x (term.unop unop.isFunc f & prop.forallc fx f forallp'), from free_in_prop.and₁ this,
+  --         have free_in_prop x (term.unop unop.isFunc f && prop.forallc fx f forallp'), from free_in_prop.and₁ this,
   --         have free_in_prop x (spec.func f fx S₆ S₇).to_prop, from h₃ ▸ this,
   --         show x ≠ y ∧ free_in_prop x (spec.func f fx S₆ S₇).to_prop, from ⟨x_neq_y, this⟩
   --       ) (
@@ -396,7 +487,7 @@ lemma free_of_subst_spec {R: spec} {x y: var} {v: value}:
   --           have free_in_term x f, from (free_of_subst_term this).right,
   --           have free_in_term x (term.unop unop.isFunc f), from free_in_term.unop this,
   --           have free_in_prop x (term.unop unop.isFunc f), from free_in_prop.term this,
-  --           have free_in_prop x (term.unop unop.isFunc f & prop.forallc fx f forallp'), from free_in_prop.and₁ this,
+  --           have free_in_prop x (term.unop unop.isFunc f && prop.forallc fx f forallp'), from free_in_prop.and₁ this,
   --           have free_in_prop x (spec.func f fx S₆ S₇).to_prop, from h₃ ▸ this,
   --           show x ≠ y ∧ free_in_prop x (spec.func f fx S₆ S₇).to_prop, from ⟨x_neq_y, this⟩
   --         ) (
@@ -411,7 +502,7 @@ lemma free_of_subst_spec {R: spec} {x y: var} {v: value}:
   --               have free_in_prop x (prop.implies S₆.to_prop (prop.pre f fx)), from free_in_prop.or₁ this,
   --               have free_in_prop x forallp', from free_in_prop.and₁ this,
   --               have free_in_prop x (prop.forallc fx f forallp'), from free_in_prop.forallc₂ x_neq_fx this,
-  --               have free_in_prop x (term.unop unop.isFunc f & prop.forallc fx f forallp'), from free_in_prop.and₂ this,
+  --               have free_in_prop x (term.unop unop.isFunc f && prop.forallc fx f forallp'), from free_in_prop.and₂ this,
   --               have free_in_prop x (spec.func f fx S₆ S₇).to_prop, from h₃ ▸ this,
   --               show x ≠ y ∧ free_in_prop x (spec.func f fx S₆ S₇).to_prop, from ⟨x_neq_y, this⟩
   --             ) (
@@ -422,7 +513,7 @@ lemma free_of_subst_spec {R: spec} {x y: var} {v: value}:
   --                 have free_in_term x f, from (free_of_subst_term this).right,
   --                 have free_in_term x (term.unop unop.isFunc f), from free_in_term.unop this,
   --                 have free_in_prop x (term.unop unop.isFunc f), from free_in_prop.term this,
-  --                 have free_in_prop x (term.unop unop.isFunc f & prop.forallc fx f forallp'), from free_in_prop.and₁ this,
+  --                 have free_in_prop x (term.unop unop.isFunc f && prop.forallc fx f forallp'), from free_in_prop.and₁ this,
   --                 have free_in_prop x (spec.func f fx S₆ S₇).to_prop, from h₃ ▸ this,
   --                 show x ≠ y ∧ free_in_prop x (spec.func f fx S₆ S₇).to_prop, from ⟨x_neq_y, this⟩
   --               ) (
@@ -433,10 +524,10 @@ lemma free_of_subst_spec {R: spec} {x y: var} {v: value}:
   --             )
   --           )
   --           (
-  --             assume : free_in_prop x (prop.implies ((spec.subst y v S₆).to_prop & prop.post (term.subst y v f) fx)
+  --             assume : free_in_prop x (prop.implies ((spec.subst y v S₆).to_prop && prop.post (term.subst y v f) fx)
   --                                                    (spec.subst y v S₇).to_prop),
   --             or.elim (free_in_prop.implies.inv this) (
-  --               assume : free_in_prop x ((spec.subst y v S₆).to_prop & prop.post (term.subst y v f) fx),
+  --               assume : free_in_prop x ((spec.subst y v S₆).to_prop && prop.post (term.subst y v f) fx),
   --               or.elim (free_in_prop.and.inv this) (
   --                 assume : free_in_prop x (spec.subst y v S₆).to_prop,
   --                 have x_neq_y: x ≠ y, from (S₆_ih this).left,
@@ -445,7 +536,7 @@ lemma free_of_subst_spec {R: spec} {x y: var} {v: value}:
   --                 have free_in_prop x (prop.implies S₆.to_prop (prop.pre f fx)), from free_in_prop.or₁ this,
   --                 have free_in_prop x forallp', from free_in_prop.and₁ this,
   --                 have free_in_prop x (prop.forallc fx f forallp'), from free_in_prop.forallc₂ x_neq_fx this,
-  --                 have free_in_prop x (term.unop unop.isFunc f & prop.forallc fx f forallp'), from free_in_prop.and₂ this,
+  --                 have free_in_prop x (term.unop unop.isFunc f && prop.forallc fx f forallp'), from free_in_prop.and₂ this,
   --                 have free_in_prop x (spec.func f fx S₆ S₇).to_prop, from h₃ ▸ this,
   --                 show x ≠ y ∧ free_in_prop x (spec.func f fx S₆ S₇).to_prop, from ⟨x_neq_y, this⟩
   --               ) (
@@ -456,7 +547,7 @@ lemma free_of_subst_spec {R: spec} {x y: var} {v: value}:
   --                   have free_in_term x f, from (free_of_subst_term this).right,
   --                   have free_in_term x (term.unop unop.isFunc f), from free_in_term.unop this,
   --                   have free_in_prop x (term.unop unop.isFunc f), from free_in_prop.term this,
-  --                   have free_in_prop x (term.unop unop.isFunc f & prop.forallc fx f forallp'), from free_in_prop.and₁ this,
+  --                   have free_in_prop x (term.unop unop.isFunc f && prop.forallc fx f forallp'), from free_in_prop.and₁ this,
   --                   have free_in_prop x (spec.func f fx S₆ S₇).to_prop, from h₃ ▸ this,
   --                   show x ≠ y ∧ free_in_prop x (spec.func f fx S₆ S₇).to_prop, from ⟨x_neq_y, this⟩
   --                 ) (
@@ -469,11 +560,11 @@ lemma free_of_subst_spec {R: spec} {x y: var} {v: value}:
   --               assume : free_in_prop x (spec.subst y v S₇).to_prop,
   --               have x_neq_y: x ≠ y, from (S₇_ih this).left,
   --               have free_in_prop x S₇.to_prop, from (S₇_ih this).right,
-  --               have free_in_prop x (prop.implies (S₆.to_prop & prop.post f fx)
+  --               have free_in_prop x (prop.implies (S₆.to_prop && prop.post f fx)
   --                                                  S₇.to_prop), from free_in_prop.or₂ this,
   --               have free_in_prop x forallp', from free_in_prop.and₂ this,
   --               have free_in_prop x (prop.forallc fx f forallp'), from free_in_prop.forallc₂ x_neq_fx this,
-  --               have free_in_prop x (term.unop unop.isFunc f & prop.forallc fx f forallp'), from free_in_prop.and₂ this,
+  --               have free_in_prop x (term.unop unop.isFunc f && prop.forallc fx f forallp'), from free_in_prop.and₂ this,
   --               have free_in_prop x (spec.func f fx S₆ S₇).to_prop, from h₃ ▸ this,
   --               show x ≠ y ∧ free_in_prop x (spec.func f fx S₆ S₇).to_prop, from ⟨x_neq_y, this⟩
   --             )
@@ -485,10 +576,32 @@ lemma free_of_subst_spec {R: spec} {x y: var} {v: value}:
 
 lemma free_of_subst_env_spec {R: spec} {σ: env} {x y: var} {v: value}:
         free_in_prop x (spec.subst_env (σ[y↦v]) R).to_prop → x ≠ y ∧ free_in_prop x (spec.subst_env σ R).to_prop :=
+
   assume x_free: free_in_prop x (spec.subst_env (σ[y↦v]) R).to_prop,
-  have spec.subst_env (σ[y↦v]) R = spec.subst y v (spec.subst_env σ R), by unfold spec.subst_env,
-  have free_in_prop x (spec.subst y v (spec.subst_env σ R)).to_prop, from this ▸ x_free,
-  show x ≠ y ∧ free_in_prop x (spec.subst_env σ R), from free_of_subst_spec this
+  show x ≠ y ∧ free_in_prop x (spec.subst_env σ R), by begin
+    induction σ with z v' σ' ih,
+    show x ≠ y ∧ free_in_prop x (spec.subst_env env.empty R), from (
+      have spec.subst_env (env.empty[y↦v]) R = spec.subst_env env.empty (spec.subst y v R), by unfold spec.subst_env,
+      have x_free': free_in_prop x (spec.subst_env env.empty (spec.subst y v R)).to_prop, from this ▸ x_free,
+      have (spec.subst_env env.empty (spec.subst y v R))
+         = (spec.subst y v R), by unfold spec.subst_env,
+      have free_in_prop x (spec.to_prop (spec.subst y v R)), from this ▸ x_free',
+      have h: x ≠ y ∧ free_in_prop x R, from free_of_subst_spec this,
+      have (spec.subst_env env.empty R) = R, by unfold spec.subst_env,
+      show x ≠ y ∧ free_in_prop x (spec.subst_env env.empty R), from ⟨h.left, this.symm ▸ h.right⟩
+    ),
+    show x ≠ y ∧ free_in_prop x (spec.subst_env (σ'[z↦v']) R), from (
+      have spec.subst_env (σ'[z↦v'][y↦v]) R = spec.subst_env (σ'[z↦v']) (spec.subst y v R), by unfold spec.subst_env,
+      have x_free': free_in_prop x (spec.subst_env (σ'[z↦v']) (spec.subst y v R)).to_prop, from this ▸ x_free,
+
+      -- ih
+
+      -- free_of_subst_spec
+
+      
+
+    )
+  end
 
 lemma free_of_subst_env {R: spec} {σ: env} {x: var}:
         free_in_prop x (spec.subst_env σ R).to_prop → free_in_prop x R.to_prop :=
@@ -505,34 +618,145 @@ lemma free_of_subst_env {R: spec} {σ: env} {x: var}:
     )
   end
 
+lemma term.subst_env.var {σ: env} {x: var} {v: value}:
+      σ x = some v → (term.subst_env σ x = v) :=
+begin
+  intro env_has_x,
+  induction σ with y v' σ' ih,
+  show (term.subst_env env.empty x = v), by begin
+    have env_has_none: (env.apply env.empty x = none), by unfold env.apply,
+    have : (some v = none), from env_has_x ▸ env_has_none,
+    contradiction
+  end,
+  show (term.subst_env (σ'[y↦v']) x = v), from
+    have app: ((σ'[y↦v']).apply x = (if y = x then v' else σ'.apply x)), by unfold env.apply,
+    if x_eq_y: x = y then
+      have (y = x) = «true», by simp [x_eq_y],
+      have ((σ'[y↦v']).apply x = v'), by simp * at *,
+      have some v' = some v, from eq.trans this.symm env_has_x,
+      have v'_is_v: v' = v, by injection this,
+      have term.subst_env (σ'[y↦v']) x = term.subst y v' (term.subst_env σ' x),
 
-lemma qfprop.subst_env.and {σ: env} {P Q: qfprop}:
-      qfprop.subst_env σ (P & Q) = (qfprop.subst_env σ P & qfprop.subst_env σ Q) :=
+
+      -- from eq. -- x_eq_y ▸ app,
+      -- have env_has_none: (σ'[y↦v']).apply x = v',
+      sorry
+
+    else
+      sorry
+    -- calc
+    -- vc.subst_env (σ'[x↦v]) P.not = vc.subst x v (vc.subst_env σ' P.not) : by unfold vc.subst_env
+    --                          ... = vc.subst x v (vc.subst_env σ' P).not : by rw[ih]
+    --                          ... = (vc.subst x v (vc.subst_env σ' P)).not : by unfold vc.subst
+    --                          ... = (vc.subst_env (σ'[x↦v]) P).not : by unfold vc.subst_env
+end
+
+lemma vc.subst_env.not {σ: env} {P: vc}:
+      vc.subst_env σ P.not = (vc.subst_env σ P).not :=
 begin
   induction σ with x v σ' ih,
-  show (qfprop.subst_env env.empty (P & Q) = (qfprop.subst_env env.empty P & qfprop.subst_env env.empty Q)), by begin
-    have h1: (qfprop.subst_env env.empty P = P), by unfold qfprop.subst_env,
-    have h2: (qfprop.subst_env env.empty Q = Q), by unfold qfprop.subst_env,
+  show (vc.subst_env env.empty P.not = (vc.subst_env env.empty P).not), by begin
     calc
-      qfprop.subst_env env.empty (P & Q) = (P & Q) : by unfold qfprop.subst_env
-                                      ... = (qfprop.subst_env env.empty P & Q) : by rw[h1]
-                                      ... = (qfprop.subst_env env.empty P & qfprop.subst_env env.empty Q) : by rw[h2]
+      vc.subst_env env.empty P.not = P.not : by unfold vc.subst_env
+                               ... = (vc.subst_env env.empty P).not : by unfold vc.subst_env
   end,
-  show (qfprop.subst_env (σ'[x↦v]) (P & Q) = (qfprop.subst_env (σ'[x↦v]) P & qfprop.subst_env (σ'[x↦v]) Q)), by begin
-    have h1: (qfprop.subst x v (qfprop.subst_env σ' P) = qfprop.subst_env (σ'[x↦v]) P), by unfold qfprop.subst_env,
+  show (vc.subst_env (σ'[x↦v]) P.not = (vc.subst_env (σ'[x↦v]) P).not), by begin
     calc
-    qfprop.subst_env (σ'[x↦v]) (P & Q) = qfprop.subst x v (qfprop.subst_env σ' (P & Q)) : by unfold qfprop.subst_env
-                                   ... = qfprop.subst x v (qfprop.subst_env σ' P & qfprop.subst_env σ' Q) : by rw[ih]
-                                   ... = (qfprop.subst x v (qfprop.subst_env σ' P) &
-                                          qfprop.subst x v (qfprop.subst_env σ' Q)) : by refl
-                                   ... = (qfprop.subst_env (σ'[x↦v]) P &
-                                          qfprop.subst x v (qfprop.subst_env σ' Q)) : by unfold qfprop.subst_env
-                                   ... = (qfprop.subst_env (σ'[x↦v]) P & qfprop.subst_env (σ'[x↦v]) Q) : by unfold qfprop.subst_env
+    vc.subst_env (σ'[x↦v]) P.not = vc.subst x v (vc.subst_env σ' P.not) : by unfold vc.subst_env
+                             ... = vc.subst x v (vc.subst_env σ' P).not : by rw[ih]
+                             ... = (vc.subst x v (vc.subst_env σ' P)).not : by unfold vc.subst
+                             ... = (vc.subst_env (σ'[x↦v]) P).not : by unfold vc.subst_env
   end
 end
 
-lemma valid_env.and {σ: env} {P Q: qfprop}: σ ⊨ P → σ ⊨ Q → σ ⊨ (P & Q) :=
-  assume p_valid: valid (qfprop.subst_env σ P),
-  assume q_valid: valid (qfprop.subst_env σ Q),
-  have qfprop.subst_env σ (P & Q) = (qfprop.subst_env σ P & qfprop.subst_env σ Q), from qfprop.subst_env.and,
-  show σ ⊨ (P & Q), from this.symm ▸ valid.and p_valid q_valid
+lemma vc.subst_env.and {σ: env} {P Q: vc}:
+      vc.subst_env σ (P && Q) = (vc.subst_env σ P && vc.subst_env σ Q) :=
+begin
+  induction σ with x v σ' ih,
+  show (vc.subst_env env.empty (P && Q) = (vc.subst_env env.empty P && vc.subst_env env.empty Q)), by begin
+    have h1: (vc.subst_env env.empty P = P), by unfold vc.subst_env,
+    have h2: (vc.subst_env env.empty Q = Q), by unfold vc.subst_env,
+    calc
+      vc.subst_env env.empty (P && Q) = (P && Q) : by unfold vc.subst_env
+                                  ... = (vc.subst_env env.empty P && Q) : by rw[h1]
+                                  ... = (vc.subst_env env.empty P && vc.subst_env env.empty Q) : by rw[h2]
+  end,
+  show (vc.subst_env (σ'[x↦v]) (P && Q) = (vc.subst_env (σ'[x↦v]) P && vc.subst_env (σ'[x↦v]) Q)), by begin
+    have h1: (vc.subst x v (vc.subst_env σ' P) = vc.subst_env (σ'[x↦v]) P), by unfold vc.subst_env,
+    calc
+    vc.subst_env (σ'[x↦v]) (P && Q) = vc.subst x v (vc.subst_env σ' (P && Q)) : by unfold vc.subst_env
+                                ... = vc.subst x v (vc.subst_env σ' P && vc.subst_env σ' Q) : by rw[ih]
+                                ... = (vc.subst x v (vc.subst_env σ' P) &&
+                                       vc.subst x v (vc.subst_env σ' Q)) : by refl
+                                ... = (vc.subst_env (σ'[x↦v]) P &&
+                                       vc.subst x v (vc.subst_env σ' Q)) : by unfold vc.subst_env
+                                ... = (vc.subst_env (σ'[x↦v]) P && vc.subst_env (σ'[x↦v]) Q) : by unfold vc.subst_env
+  end
+end
+
+lemma vc.subst_env.or {σ: env} {P Q: vc}:
+      vc.subst_env σ (P || Q) = (vc.subst_env σ P || vc.subst_env σ Q) :=
+begin
+  induction σ with x v σ' ih,
+  show (vc.subst_env env.empty (P || Q) = (vc.subst_env env.empty P || vc.subst_env env.empty Q)), by begin
+    have h1: (vc.subst_env env.empty P = P), by unfold vc.subst_env,
+    have h2: (vc.subst_env env.empty Q = Q), by unfold vc.subst_env,
+    calc
+      vc.subst_env env.empty (P || Q) = (P || Q) : by unfold vc.subst_env
+                                  ... = (vc.subst_env env.empty P || Q) : by rw[h1]
+                                  ... = (vc.subst_env env.empty P || vc.subst_env env.empty Q) : by rw[h2]
+  end,
+  show (vc.subst_env (σ'[x↦v]) (P || Q) = (vc.subst_env (σ'[x↦v]) P || vc.subst_env (σ'[x↦v]) Q)), by begin
+    have h1: (vc.subst x v (vc.subst_env σ' P) = vc.subst_env (σ'[x↦v]) P), by unfold vc.subst_env,
+    calc
+    vc.subst_env (σ'[x↦v]) (P || Q) = vc.subst x v (vc.subst_env σ' (P || Q)) : by unfold vc.subst_env
+                                ... = vc.subst x v (vc.subst_env σ' P || vc.subst_env σ' Q) : by rw[ih]
+                                ... = (vc.subst x v (vc.subst_env σ' P) ||
+                                       vc.subst x v (vc.subst_env σ' Q)) : by refl
+                                ... = (vc.subst_env (σ'[x↦v]) P ||
+                                       vc.subst x v (vc.subst_env σ' Q)) : by unfold vc.subst_env
+                                ... = (vc.subst_env (σ'[x↦v]) P || vc.subst_env (σ'[x↦v]) Q) : by unfold vc.subst_env
+  end
+end
+
+lemma vc.subst_env.pre₁ {σ: env} {op: unop} {t: term}:
+      vc.subst_env σ (vc.pre₁ op t) = vc.pre₁ op (term.subst_env σ t) :=
+begin
+  induction σ with x v σ' ih,
+  show (vc.subst_env env.empty (vc.pre₁ op t) = vc.pre₁ op (term.subst_env env.empty t)), by begin
+    have h1: (term.subst_env env.empty t = t), by unfold term.subst_env,
+    calc
+      vc.subst_env env.empty (vc.pre₁ op t) = (vc.pre₁ op t) : by unfold vc.subst_env
+                                        ... = (vc.pre₁ op (term.subst_env env.empty t)) : by rw[h1]
+  end,
+  show (vc.subst_env (σ'[x↦v]) (vc.pre₁ op t) = vc.pre₁ op (term.subst_env (σ'[x↦v]) t)), by begin
+    calc
+    vc.subst_env (σ'[x↦v]) (vc.pre₁ op t) = vc.subst x v (vc.subst_env σ' (vc.pre₁ op t)) : by unfold vc.subst_env
+                             ... = vc.subst x v (vc.pre₁ op (term.subst_env σ' t)) : by rw[ih]
+                             ... = vc.pre₁ op (term.subst x v (term.subst_env σ' t)) : by unfold vc.subst
+                             ... = vc.pre₁ op (term.subst_env (σ'[x↦v]) t) : by unfold term.subst_env
+  end
+end
+
+lemma valid_env.and {σ: env} {P Q: vc}: σ ⊨ P → σ ⊨ Q → σ ⊨ (P && Q) :=
+  assume p_valid: valid (vc.subst_env σ P),
+  assume q_valid: valid (vc.subst_env σ Q),
+  have vc.subst_env σ (P && Q) = (vc.subst_env σ P && vc.subst_env σ Q), from vc.subst_env.and,
+  show σ ⊨ (P && Q), from this.symm ▸ valid.and p_valid q_valid
+
+lemma valid.mp_env {σ: env} {P Q: vc}: σ ⊨ vc.implies P Q → σ ⊨ P → σ ⊨ Q :=
+  assume impl: σ ⊨ (vc.implies P Q),
+  assume p: σ ⊨ P,
+  have vc.subst_env σ (vc.implies P Q) = (vc.subst_env σ P.not || vc.subst_env σ Q), from vc.subst_env.or,
+  have h: ⊨ (vc.subst_env σ P.not || vc.subst_env σ Q), from this ▸ impl,
+  have vc.subst_env σ P.not = (vc.subst_env σ P).not, from vc.subst_env.not,
+  have ⊨ ((vc.subst_env σ P).not || vc.subst_env σ Q), from this ▸ h,
+  have ⊨ vc.implies (vc.subst_env σ P) (vc.subst_env σ Q), from this,
+  show σ ⊨ Q, from valid.mp this p
+
+lemma valid.pre₁.inv {vₓ: value} {op: unop}: ⊨ vc.pre₁ op vₓ → (∃v, op vₓ = some v) :=
+  assume pre_valid: ⊨ vc.pre₁ op vₓ,
+  show (∃v, op vₓ = some v), by begin
+    cases pre_valid,
+    case valid.pre₁ v exist_v { exact exist_v }
+  end
