vcgen.lean
@@ -7,58 +7,58 @@ notation P `⊢` e `:` Q : 10 := exp.vcgen P e Q
 
 | tru {P: prop} {x: var} {e: exp} {Q: propctx}:
     x ∉ FV P →
-    (P && x ≡ value.true ⊢ e : Q) →
-    (P ⊢ lett x = true in e : propctx.exist x (x ≡ value.true & Q))
+    (P && (x ≡ value.true) ⊢ e : Q) →
+    (P ⊢ lett x = true in e : propctx.exis x ((x ≡ value.true) && Q))
 
 | fals {P: prop} {x: var} {e: exp} {Q: propctx}:
     x ∉ FV P →
-    (P & x ≡ value.false ⊢ e : Q) →
-    (P ⊢ letf x = false in e : propctx.exist x (x ≡ value.false & Q))
+    (P && (x ≡ value.false) ⊢ e : Q) →
+    (P ⊢ letf x = false in e : propctx.exis x ((x ≡ value.false) && Q))
 
 | num {P: prop} {x: var} {n: ℕ} {e: exp} {Q: propctx}:
     x ∉ FV P →
-    (P & x ≡ value.num n ⊢ e : Q) →
-    (P ⊢ letn x = n in e : propctx.exist x (x ≡ value.num n & Q))
+    (P && (x ≡ value.num n) ⊢ e : Q) →
+    (P ⊢ letn x = n in e : propctx.exis x ((x ≡ value.num n) && Q))
 
 | func {P: prop} {f x: var} {R S: spec} {e₁ e₂: exp} {Q₁ Q₂: propctx}:
     f ∉ FV P →
     x ∉ FV P →
     FV R.to_prop ⊆ FV P →
     FV S.to_prop ⊆ FV P →
-    (P & spec.func f x R S & R ⊢ e₂ : Q₂) →
-    ⟪prop.implies (P & spec.func f x R S & R & Q₂ (term.app f x)) S⟫ →
+    (P && spec.func f x R S && R ⊢ e₂ : Q₂) →
+    ⟪prop.implies (P && spec.func f x R S && R && Q₂ (term.app f x)) S⟫ →
     (P ⊢ letf f[x] req R ens S {e₁} in e₂ :
-         propctx.exist f (spec.func f x R S & Q₁))
+         propctx.exis f (spec.func f x R S && Q₁))
 
 | unop {P: prop} {op: unop} {e: exp} {x y: var} {Q: propctx}:
     x ∈ FV P →
     y ∉ FV P →
-    (P & y ≡ term.unop op x ⊢ e : Q) →
+    (P && (y ≡ term.unop op x) ⊢ e : Q) →
     ⟪ prop.implies P (prop.pre₁ op x) ⟫ →
-    (P ⊢ letop y = op [x] in e : propctx.exist y (y ≡ term.unop op x & Q))
+    (P ⊢ letop y = op [x] in e : propctx.exis y ((y ≡ term.unop op x) && Q))
 
 | binop {P: prop} {op: binop} {e: exp} {x y z: var} {Q: propctx}:
     x ∈ FV P →
     y ∈ FV P →
     z ∉ FV P →
-    (P & z ≡ term.binop op x y ⊢ e : Q) →
+    (P && (z ≡ term.binop op x y) ⊢ e : Q) →
     ⟪ prop.implies P (prop.pre₂ op x y) ⟫ →
-    (P ⊢ letop2 y = op [x, y] in e : propctx.exist y (z ≡ term.binop op x y & Q))
+    (P ⊢ letop2 y = op [x, y] in e : propctx.exis y ((z ≡ term.binop op x y) && Q))
 
 | app {P: prop} {e: exp} {y f x: var} {Q: propctx}:
     f ∈ FV P →
     x ∈ FV P →
     y ∉ FV P →
-    (P & prop.call f x & y ≡ term.app f x & prop.post f x ⊢ e : Q) →
-    ⟪ prop.implies (P & prop.call f x) (term.unop unop.isFunc f & prop.pre f x) ⟫ →
-    (P ⊢ letapp y = f [x] in e : propctx.exist y (prop.call f x & y ≡ term.app f x & prop.post f x & Q))
+    (P && prop.call f x && (y ≡ term.app f x) && prop.post f x ⊢ e : Q) →
+    ⟪ prop.implies (P && prop.call f x) (term.unop unop.isFunc f && prop.pre f x) ⟫ →
+    (P ⊢ letapp y = f [x] in e : propctx.exis y (prop.call f x && (y ≡ term.app f x) && prop.post f x && Q))
 
 | ite {P: prop} {e₁ e₂: exp} {x: var} {Q₁ Q₂: propctx}:
     x ∈ FV P →
-    (P & x ⊢ e₁ : Q₁) →
-    (P & term.unop unop.not x ⊢ e₂ : Q₂) →
+    (P && x ⊢ e₁ : Q₁) →
+    (P && term.unop unop.not x ⊢ e₂ : Q₂) →
     ⟪ prop.implies P (term.unop unop.isBool x) ⟫ →
-    (P ⊢ exp.ite x e₁ e₂ : (propctx.implies x Q₁ & propctx.implies (term.unop unop.not x) Q₂))
+    (P ⊢ exp.ite x e₁ e₂ : (propctx.implies x Q₁ && propctx.implies (term.unop unop.not x) Q₂))
 
 | return {P: prop} {x: var}:
     x ∈ FV P →
@@ -74,28 +74,28 @@ notation `⊢` σ `:` Q : 10 := env.vcgen σ Q
 
 | tru {σ: env} {x: var} {Q: prop}:
     (⊢ σ : Q) →
-    (⊢ (σ[x ↦ value.true]) : (Q & x ≡ value.true))
+    (⊢ (σ[x ↦ value.true]) : (Q && (x ≡ value.true)))
 
 | fls {σ: env} {x: var} {Q: prop}:
     (⊢ σ : Q) →
-    (⊢ (σ[x ↦ value.false]) : (Q & x ≡ value.false))
+    (⊢ (σ[x ↦ value.false]) : (Q && (x ≡ value.false)))
 
 | num {n: ℤ} {σ: env} {x: var} {Q: prop}:
     (⊢ σ : Q) →
-    (⊢ (σ[x ↦ value.num n]) : (Q & x ≡ value.num n))
+    (⊢ (σ[x ↦ value.num n]) : (Q && (x ≡ value.num n)))
 
 | func {σ₁ σ₂: env} {f g x: var} {R S: spec} {e: exp} {Q₁ Q₂: prop} {Q₃: propctx}:
     (⊢ σ₁ : Q₁) →
     (⊢ σ₂ : Q₂) →
     FV R.to_prop ⊆ FV Q₂ ∪ { g, x } →
     FV S.to_prop ⊆ FV Q₂ ∪ { g, x } →
-    (Q₂ & spec.func g x R S & R ⊢ e : Q₃) →
-    ⟪prop.implies (Q₂ & spec.func g x R S & R & Q₃ (term.app g x)) S⟫ →
+    (Q₂ && spec.func g x R S && R ⊢ e : Q₃) →
+    ⟪prop.implies (Q₂ && spec.func g x R S && R && Q₃ (term.app g x)) S⟫ →
     (⊢ (σ₁[f ↦ value.func g x R S e σ₂]) :
-      (Q₁ &
+      (Q₁ &&
        spec.func f x (spec.subst_env (σ₂[g↦value.func g x R S e σ₂]) R)
-                     (spec.subst_env (σ₂[g↦value.func g x R S e σ₂]) S) &
-       f ≡ value.func g x R S e σ₂))
+                     (spec.subst_env (σ₂[g↦value.func g x R S e σ₂]) S) &&
+       (f ≡ value.func g x R S e σ₂)))
 
 notation `⊢` σ `:` Q : 10 := env.vcgen σ Q
 
@@ -104,7 +104,7 @@ notation H `⊩` s : 10 := stack.vcgen H s
 
 | top {H: list call} {P: prop} {σ: env} {e: exp} {Q: propctx}:
     (⊢ σ : P) →
-    (H & P ⊢ e : Q) →
+    (H && P ⊢ e : Q) →
     (H ⊩ (σ, e))
 
 | cons {H: list call} {P: prop} {s: stack} {σ σ': env} {f g x y z: var} {R S: spec} {e: exp} {v: value} {Q: propctx}:
@@ -113,7 +113,7 @@ notation H `⊩` s : 10 := stack.vcgen H s
     (σ f = value.func g z R S e σ') →
     (σ x = v) →
     ((σ[g↦value.func g z R S e σ'][z↦v], e) ⟶* s) →
-    (H & P ⊢ letapp y = f[x] in e : Q) →
+    (H && P ⊢ letapp y = f[x] in e : Q) →
     (H ⊩ (s · [σ, let y = f[x] in e]))
 
 notation P `⊩` s : 10 := stack.vcgen P s
